Separate out scope checking for context

theories/Context.v
@@ -30,8 +30,15 @@ Import Map.MapNotations.
 
 Definition eq_usage Δ Δ': {Δ = Δ'} + {Δ ≠ Δ'}.
 Proof.
-  set (s := eq_use).
   decide equality.
+  destruct a as [x u], p as [y u'].
+  destruct (eq_var x y), (eq_use u u').
+  all: subst.
+  all: auto.
+  all: right.
+  all: intro p.
+  all: inversion p.
+  all: auto.
 Defined.
 
 Lemma length_xsof {Γ}: length (xsof Γ) = length Γ.
@@ -44,178 +51,287 @@ Proof.
   auto.
 Qed.
 
-Lemma length_same_lmem_l {x xs Δ Δ'}: lmem x xs Δ Δ' → length xs = length Δ.
-Proof.
-  intro p.
-  induction p.
-  all: cbn.
-  all: auto.
-Qed.
-
-Lemma length_same_lmem_r {x xs Δ Δ'}: lmem x xs Δ Δ' → length xs = length Δ'.
-Proof.
-  intro p.
-  induction p.
-  all: cbn.
-  all: auto.
-Qed.
-
 Section Typecheck.
   Import OptionNotations.
 
-  Function lookup x Γ Δ :=
-    match Γ, Δ with
-    | cons (y, t) Γ', cons u Δ' =>
+  Function lookup x Δ :=
+    if Δ is cons (y, u) Δ'
+    then
         if eq_var x y
         then
           if u is u_unused
           then
-            if Nat.eq_dec (length Γ') (length Δ')
-            then
-              Some (cons u_used Δ', t)
-            else
-              None
+             Some (cons (y, u_used) Δ')
           else
             None
         else
-          do ' (Δ'', t)  ← lookup x Γ' Δ' ;
-          Some (cons u Δ'', t)
-    | _, _ => None
-    end.
+          do Δ'' ← lookup x Δ' ;
+          Some (cons (y, u) Δ'')
+  else
+    None.
 
-  Function typecheck Γ Δ E t: option usage :=
-    match E, t with
-    | E_lam x E, t1 * t2 =>
-        do ' (u_used :: Δ') ← typecheck ((x, t1) :: Γ) (u_unused :: Δ) E t2 ;
-        Some Δ'
-
-    | E_tt, t_unit =>
-        if Nat.eq_dec (length Γ) (length Δ)
+  Function usecheck Δ E: option usage :=
+    match E with
+    | E_lam x E =>
+        do ' ((y, u_used) :: Δ') ← usecheck ((x, u_unused) :: Δ) E ;
+        if eq_var x y
         then
-          Some Δ
+          Some Δ'
         else
           None
 
-    | E_fanout E E', t1 * t2 =>
-        do Δ1 ← typecheck Γ Δ E t1 ;
-        do Δ2 ← typecheck Γ Δ1 E' t2 ;
+    | E_tt => Some Δ
+
+    | E_fanout E E' =>
+        do Δ1 ← usecheck Δ E ;
+        do Δ2 ← usecheck Δ1 E' ;
         Some Δ2
 
-    | E_neu e, _ =>
-        do ' (Δ, t') ← typeinfer Γ Δ e ;
-        if eq_type t t' then Some Δ else None
+    | E_neu e =>
+        useinfer Δ e
 
-    | _, _ => None
     end
       %list
-  with typeinfer Γ Δ e: option (usage * type) :=
+  with useinfer Δ e: option usage :=
     match e with
-    | e_var x => lookup x Γ Δ
+    | e_var x => lookup x Δ
 
     | e_app e E' =>
-        do ' (Δ1, t1 * t2) ← typeinfer Γ Δ e ;
-        do Δ2 ← typecheck Γ Δ1 E' t1 ;
-        Some (Δ2, t2)
+        do Δ1 ← useinfer Δ e ;
+        do Δ2 ← usecheck Δ1 E' ;
+        Some Δ2
 
     | e_step e E' t =>
-        do ' (Δ1, t_unit) ← typeinfer Γ Δ e ;
-        do Δ2 ← typecheck Γ Δ1 E' t ;
-        Some (Δ2, t)
+        do Δ1 ← useinfer Δ e ;
+        do Δ2 ← usecheck Δ1 E' ;
+        Some Δ2
 
     | e_let x y e E' t3 =>
-        do ' (Δ1, t1 * t2) ← typeinfer Γ Δ e ;
-        do ' (u_used :: u_used :: Δ2) ← typecheck ((y, t2) :: (x, t1) :: Γ) (u_unused :: u_unused :: Δ1) E' t3 ;
-        Some (Δ2, t3)
+        do Δ1 ← useinfer Δ e ;
+        do ' ((y', u_used) :: (x', u_used) :: Δ2) ← usecheck ((y, u_unused) :: (x, u_unused) :: Δ1) E' ;
+        match eq_var x x', eq_var y y' with
+        | left _, left _ => Some Δ2
+        | _, _ => None
+        end
 
     | e_cut E t =>
-        do Δ ← typecheck Γ Δ E t ;
-        Some (Δ, t)
+        do Δ ← usecheck Δ E ;
+        Some Δ
+    end
+      %list.
+
+  Function typecheck Γ E t: bool :=
+    match E, t with
+    | E_lam x E, t1 * t2 =>
+        typecheck ((x, t1) :: Γ) E t2
+
+    | E_tt, t_unit => true
+
+    | E_fanout E E', t1 * t2 =>
+        typecheck Γ E t1
+        && typecheck Γ E' t2
+
+    | E_neu e, _ =>
+        if typeinfer Γ e is Some t'
+        then
+          if eq_type t t' then true else false
+        else
+          false
+
+    | _, _ => false
+    end
+     %bool %list
+  with typeinfer Γ e: option type :=
+    match e with
+    | e_var x => find x Γ
+
+    | e_app e E' =>
+        do ' (t1 * t2) ← typeinfer Γ e ;
+        if typecheck Γ E' t1
+        then
+          Some t2
+        else
+          None
+
+    | e_step e E' t =>
+        do ' t_unit ← typeinfer Γ e ;
+        if typecheck Γ E' t
+        then
+          Some t
+        else
+          None
+
+    | e_let x y e E' t3 =>
+        do ' (t1 * t2) ← typeinfer Γ e ;
+        if typecheck ((y, t2) :: (x, t1) :: Γ) E' t3
+        then
+          Some t3
+        else
+          None
+
+    | e_cut E t =>
+        if typecheck Γ E t
+        then
+          Some t
+        else
+          None
     end
       %list.
 End Typecheck.
 
 Fixpoint
-  typecheck_sound {E} {struct E}:
-  ∀ {Γ Δ Δ' t}, typecheck Γ Δ E t = Some Δ' → check Γ Δ Δ' E t
+  usecheck_sound {E} {struct E}:
+  ∀ {Δ Δ'}, usecheck Δ E = Some Δ' → sE Δ Δ' E
     with
-  typeinfer_sound {e} {struct e}:
-  ∀ {Γ Δ Δ' t}, typeinfer Γ Δ e = Some (Δ', t) → infer Γ Δ Δ' e t
-
+  useinfer_sound {e} {struct e}:
+  ∀ {Δ Δ'}, useinfer Δ e = Some Δ' → se Δ Δ' e
 .
 Proof using.
   - destruct E.
     all: cbn.
-    all: intros ? ? ? ? p.
+    all: intros ? ? p.
     all: inversion p.
     all: subst.
     all: clear p.
-    + destruct t.
-      all: try discriminate.
-      destruct typecheck eqn:q.
+    + destruct usecheck eqn:q.
       2: discriminate.
       destruct u.
       1: discriminate.
-      destruct u.
+      destruct p.
+      destruct u0.
+      2: discriminate.
+      destruct eq_var.
       2: discriminate.
       inversion H0.
       subst.
       constructor.
       auto.
-    + destruct t.
-      all: try discriminate.
-      destruct Nat.eq_dec.
+    + constructor.
+    + destruct usecheck eqn:q1.
       2: discriminate.
-      inversion H0.
-      subst.
-      constructor.
-      auto.
-    + destruct t.
-      all: try discriminate.
-      destruct typecheck eqn:q1.
-      2: discriminate.
-      destruct typecheck eqn:q2 in H0.
+      destruct usecheck eqn:q2 in H0.
       2: discriminate.
       inversion H0.
       subst.
       econstructor.
       all: eauto.
     + constructor.
-      destruct typeinfer eqn:q.
-      2: discriminate.
-      destruct p.
-      destruct eq_type.
-      2: discriminate.
-      inversion H0.
-      subst.
-      eauto.
+      apply useinfer_sound.
+      all: auto.
   - destruct e.
     all: cbn.
-    all: intros ? ? ? ? p.
+    all: intros ? ? p.
     all: inversion p.
     all: subst.
     all: clear p.
     + constructor.
-      * generalize dependent Δ'.
-        functional induction (lookup x Γ Δ).
-        all: cbn.
-        all: intros ? p.
-        all: inversion p.
-        all: subst.
-        all: constructor.
-        all: eauto.
-      * generalize dependent Δ'.
-        functional induction (lookup x Γ Δ).
-        all: cbn.
-        all: intros ? p.
-        all: inversion p.
-        all: subst.
-        all: constructor.
-        all: eauto.
-        rewrite length_xsof.
+      generalize dependent Δ'.
+      functional induction (lookup x Δ).
+      all: cbn.
+      all: intros ? p.
+      all: inversion p.
+      all: subst.
+      all: constructor.
+      all: eauto.
+    + destruct useinfer eqn:q1.
+      2: discriminate.
+      destruct usecheck eqn:q2.
+      2: discriminate.
+      inversion H0.
+      subst.
+      econstructor.
+      all: eauto.
+    + destruct useinfer eqn:q1.
+      2: discriminate.
+      destruct usecheck eqn:q2.
+      2: discriminate.
+      inversion H0.
+      subst.
+      econstructor.
+      all: eauto.
+    + destruct useinfer eqn:q1.
+      2: discriminate.
+      destruct usecheck eqn:q2.
+      2: discriminate.
+      destruct u0.
+      1: discriminate.
+      destruct p.
+      destruct u1.
+      2: discriminate.
+      destruct u0.
+      1: discriminate.
+      destruct p.
+      destruct u1.
+      2: discriminate.
+      destruct eq_var.
+      2: discriminate.
+      destruct eq_var.
+      2: discriminate.
+      inversion H0.
+      subst.
+      econstructor.
+      all: eauto.
+    + destruct usecheck eqn:q.
+      2: discriminate.
+      inversion H0.
+      subst.
+      constructor.
+      eauto.
+Qed.
+
+Fixpoint
+  typecheck_sound {E} {struct E}:
+  ∀ {Γ t}, Bool.Is_true (typecheck Γ E t) → check Γ E t
+    with
+  typeinfer_sound {e} {struct e}:
+  ∀ {Γ t}, typeinfer Γ e = Some t → infer Γ e t.
+Proof using.
+  - destruct E.
+    all: cbn.
+    all: intros ? ? p.
+    all: try contradiction.
+    + destruct t.
+      all: try contradiction.
+      destruct typecheck eqn:q.
+      2: contradiction.
+      constructor.
+      apply typecheck_sound.
+      rewrite q.
+      auto.
+    + destruct t.
+      all: try contradiction.
+      constructor.
+    + destruct t.
+      all: try contradiction.
+      destruct typecheck eqn:q1.
+      2: contradiction.
+      destruct typecheck eqn:q2 in p.
+      2: contradiction.
+      constructor.
+      * apply typecheck_sound.
+        rewrite q1.
         auto.
+      * apply typecheck_sound.
+        rewrite q2.
+        auto.
+    + constructor.
+      destruct typeinfer eqn:q.
+      2: contradiction.
+      destruct eq_type.
+      2: contradiction.
+      subst.
+      auto.
+  - destruct e.
+    all: cbn.
+    all: intros ? ? p.
+    all: inversion p.
+    all: subst.
+    all: clear p.
+    + constructor.
+      apply find_sound.
+      auto.
     + destruct typeinfer eqn:q1.
       2: discriminate.
-      destruct p.
       destruct t0.
       all: try discriminate.
       destruct typecheck eqn:q2.
@@ -224,9 +340,12 @@ Proof using.
       subst.
       econstructor.
       all: eauto.
+      apply typecheck_sound.
+      rewrite q2.
+      cbv.
+      auto.
     + destruct typeinfer eqn:q1.
       2: discriminate.
-      destruct p.
       destruct t1.
       all: try discriminate.
       destruct typecheck eqn:q2.
@@ -235,75 +354,92 @@ Proof using.
       subst.
       econstructor.
       all: eauto.
+      apply typecheck_sound.
+      rewrite q2.
+      cbv.
+      auto.
     + destruct typeinfer eqn:q1.
       2: discriminate.
-      destruct p.
       destruct t1.
       all: try discriminate.
       destruct typecheck eqn:q2.
-      2: discriminate.
-      destruct u0.
-      1: discriminate.
-      destruct u0.
-      2: discriminate.
-      destruct u1.
-      1: discriminate.
-      destruct u0.
       2: discriminate.
       inversion H0.
       subst.
       econstructor.
       all: eauto.
+      apply typecheck_sound.
+      rewrite q2.
+      cbv.
+      auto.
     + destruct typecheck eqn:q.
       2: discriminate.
       inversion H0.
       subst.
       constructor.
-      eauto.
+      apply typecheck_sound.
+      rewrite q.
+      apply I.
 Qed.
 
-Fixpoint typecheck_complete {Γ E Δ Δ' t} (p: check Γ Δ Δ' E t):
-  typecheck Γ Δ E t = Some Δ'
-with
-typeinfer_complete {Γ e Δ Δ' t} (p: infer Γ Δ Δ' e t):
-  typeinfer Γ Δ e = Some (Δ', t).
+Fixpoint usecheck_complete {E Δ Δ'} (p: sE Δ Δ' E):
+  usecheck Δ E = Some Δ'
+with useinfer_complete {e Δ Δ'} (p: se Δ Δ' e):
+  useinfer Δ e = Some Δ'.
 Proof using.
   - destruct p.
     all: cbn.
-    all: try rewrite (typecheck_complete _ _ _ _ _ p).
-    all: try rewrite (typecheck_complete _ _ _ _ _ p1).
-    all: try rewrite (typecheck_complete _ _ _ _ _ p2).
-    all: try rewrite (typeinfer_complete _ _ _ _ _ H).
+    all: try rewrite (usecheck_complete _ _ _ p).
+    all: try rewrite (usecheck_complete _ _ _ p1).
+    all: try rewrite (usecheck_complete _ _ _ p2).
+    all: try rewrite (useinfer_complete _ _ _ H).
     all: auto.
-    + destruct Nat.eq_dec.
-      2: contradiction.
-      auto.
-    + destruct eq_type.
-      2: contradiction.
-      auto.
+    destruct eq_var.
+    2: contradiction.
+    auto.
   - destruct p.
     all: cbn.
-    all: try rewrite (typeinfer_complete _ _ _ _ _ p).
-    all: try rewrite (typecheck_complete _ _ _ _ _ H).
+    all: try rewrite (useinfer_complete _ _ _ p).
+    all: try rewrite (usecheck_complete _ _ _ H).
     all: auto.
-    + generalize dependent Δ'.
-      generalize dependent Δ.
-      induction H.
+    + induction H.
       all: cbn.
-      all: intros ? ? q.
-      all: inversion q.
-      all: subst.
-      all: cbn.
-      all: try contradiction.
-      all: destruct eq_var.
-      all: try contradiction.
-      * rewrite <- H1.
-        rewrite length_xsof.
-        destruct Nat.eq_dec.
+      * destruct eq_var.
         2: contradiction.
         auto.
-      * rewrite (IHmem _ _ H7).
+      * destruct eq_var.
+        1: subst; contradiction.
+        rewrite IHlmem.
         auto.
+    + destruct eq_var.
+      2: contradiction.
+      destruct eq_var.
+      2: contradiction.
+      auto.
+Qed.
+
+Fixpoint typecheck_complete {Γ E t} (p: check Γ E t):
+  typecheck Γ E t = true
+with typeinfer_complete {Γ e t} (p: infer Γ e t):
+  typeinfer Γ e = Some t.
+Proof using.
+  - destruct p.
+    all: cbn.
+    all: try rewrite (typecheck_complete _ _ _ p).
+    all: try rewrite (typecheck_complete _ _ _ p1).
+    all: try rewrite (typecheck_complete _ _ _ p2).
+    all: try rewrite (typeinfer_complete _ _ _ H).
+    all: auto.
+    destruct eq_type.
+    2: contradiction.
+    auto.
+  - destruct p.
+    all: cbn.
+    all: try rewrite (typeinfer_complete _ _ _ p).
+    all: try rewrite (typecheck_complete _ _ _ H).
+    all: auto.
+    apply find_complete.
+    auto.
 Qed.
 
 Notation "'do' n ← e0 ; e1" :=
@@ -594,9 +730,18 @@ Record span := {
   π2: s → intro ;
 }.
 
-Definition useonce Γ u: usage := List.map (λ '(x, t), u) Γ.
+Definition useonce Γ u: usage := List.map (λ '(x, t), (x, u)) Γ.
 
-Definition oftype Γ t := { E | check Γ (useonce Γ u_unused) (useonce Γ u_used) E t }.
+Definition oftype Γ t :=
+  { E |
+    Bool.Is_true (
+        typecheck Γ E t
+        && if usecheck (useonce Γ u_unused) E is Some Δ
+           then
+             if eq_usage Δ (useonce Γ u_used) then true else false
+           else
+             false)
+  }.
 
 Record iso A B := {
     to: A → B ;
